Utilities/Misc.thy
@@ -1,5 +1,5 @@
 theory Misc
-imports Main
+imports Index
 begin
 
 primrec map_fst :: "('a \<Rightarrow> 'c) \<Rightarrow> 'a \<times> 'b \<Rightarrow> 'c \<times> 'b" where
@@ -17,5 +17,40 @@ lemma [simp]: "(x::nat) \<ge> y \<Longrightarrow> \<exists>z. x = y + z"
 
 lemma [simp]: "(\<forall>x y. f x = f y \<longrightarrow> x = y) \<Longrightarrow> index_of (f a) (map f as) = index_of a as"
   by (induction as) simp_all
+
+lemma [simp]: "a \<notin> set as \<Longrightarrow> length (filter (\<lambda>x. x \<noteq> a) as) = length as"
+  by (induction as) auto
+
+lemma filter_length: "distinct as \<Longrightarrow> a \<in> set as \<Longrightarrow> 
+    length as = Suc (length (filter (\<lambda>x. x \<noteq> a) as))"
+  by (induction as) auto
+
+lemma [elim]: "distinct xs \<Longrightarrow> k < length xs \<Longrightarrow> \<forall>x\<in>set xs. x < length xs \<Longrightarrow> k \<in> set xs"
+  proof (induction "length xs" arbitrary: k xs)
+  case 0
+    thus ?case by (cases xs) simp_all
+  next case (Suc l)
+    then obtain x xs' where X: "xs = x # xs'" by (cases xs) simp_all
+    thus ?case 
+      proof (cases "x = k")
+      case False
+        from Suc X have A: "l = length (map (decr x) xs')" by simp 
+        from Suc X have B: "distinct (map (decr x) xs')" by simp 
+        from Suc X False have C: "decr x k < length (map (decr x) xs')" by simp 
+        have "\<forall>y \<in> set (map (decr x) xs'). y < length (map (decr x) xs')" 
+          proof
+            fix y
+            assume "y \<in> set (map (decr x) xs')"
+            then obtain z where Z: "z : set xs' \<and> y = decr x z" by auto
+            with Suc X have "x \<noteq> z" by auto
+            with Suc X Z show "y < length (map (decr x) xs')" by simp
+          qed
+        with Suc(1) A B C have "decr x k \<in> set (map (decr x) xs')" by fastforce
+        with Suc X False show ?thesis by simp
+      qed simp_all
+  qed
+
+lemma pack_pigeonholes: "distinct xs \<Longrightarrow> k = length xs \<Longrightarrow> \<forall>x \<in> set xs. x < k \<Longrightarrow> set xs = {x. x < k}"
+  by auto
 
 end
